src/program_proof/tulip/program/replica/replica_apply.v
@@ -5,6 +5,65 @@ From Perennial.program_proof.tulip.program.replica Require Import
 Section program.
   Context `{!heapGS Σ, !tulip_ghostG Σ}.
 
+  Theorem wp_Replica__apply__replaying
+    rp cmd pwrsS clog ilog gid γ α :
+    let clog' := clog ++ [cmd] in
+    Forall (λ nc, (nc.1 <= length clog)%nat) ilog ->
+    valid_ccommand gid cmd ->
+    group_histm_lbs_from_log γ gid clog' -∗
+    is_replica_idx rp γ α -∗
+    {{{ own_pwrs_slice pwrsS cmd ∗
+        own_replica_replaying rp clog ilog α
+    }}}
+      Replica__apply #rp (ccommand_to_val pwrsS cmd)
+    {{{ RET #();
+        own_pwrs_slice pwrsS cmd ∗
+        own_replica_replaying rp clog' ilog α
+    }}}.
+  Proof.
+    iIntros (clog' Hvicmds Hvcmd) "#Hsafe #Hidx".
+    iIntros (Φ) "!> [Hpwrs Hrp] HΦ".
+    wp_rec.
+
+    (*@ func (rp *Replica) apply(cmd txnlog.Cmd) {                              @*)
+    (*@     if cmd.Kind == 1 {                                                  @*)
+    (*@         rp.applyCommit(cmd.Timestamp, cmd.PartialWrites)                @*)
+    (*@     } else if cmd.Kind == 2 {                                           @*)
+    (*@         rp.applyAbort(cmd.Timestamp)                                    @*)
+    (*@     }                                                                   @*)
+    (*@ }                                                                       @*)
+    wp_pures.
+    destruct cmd eqn:Hcmd; wp_pures.
+    { (* Case: CmdCommit. *)
+      destruct Hvcmd as [Hvts Hvpwrs].
+      iDestruct "Hpwrs" as (pwrsL) "Hpwrs".
+      wp_apply (wp_Replica__applyCommit__replaying with "[Hsafe] Hidx [$Hpwrs $Hrp]").
+      { apply Hvicmds. }
+      { apply Hvpwrs. }
+      { rewrite uint_nat_W64_of_nat; first done. rewrite /valid_ts in Hvts. word. }
+      iIntros "[Hpwrs Hrp]".
+      wp_pures.
+      iApply "HΦ".
+      rewrite uint_nat_W64_of_nat; last first.
+      { rewrite /valid_ts in Hvts. word. }
+      by iFrame.
+    }
+    { (* Case: CmdAbort. *)
+      simpl in Hvcmd.
+      rewrite /group_histm_lbs_from_log.
+      destruct (apply_cmds clog') as [cpm histm |] eqn:Happly; last done.
+      wp_apply (wp_Replica__applyAbort__replaying with "Hrp").
+      { apply Hvicmds. }
+      { rewrite uint_nat_W64_of_nat; first by rewrite Happly. rewrite /valid_ts in Hvcmd. word. }
+      iIntros "Hrp".
+      wp_pures.
+      iApply "HΦ".
+      rewrite uint_nat_W64_of_nat; last first.
+      { rewrite /valid_ts in Hvcmd. word. }
+      by iFrame.
+    }
+  Qed.
+
   Theorem wp_Replica__apply
     rp cmd pwrsS cloga gid rid γ α :
     let cloga' := cloga ++ [cmd] in
