src/program_proof/tulip/program/replica/replica_apply_commit.v
@@ -5,6 +5,139 @@ From Perennial.program_proof.tulip.program.replica Require Import
 Section program.
   Context `{!heapGS Σ, !tulip_ghostG Σ}.
 
+  Theorem wp_Replica__applyCommit__replaying
+    rp (tsW : u64) pwrsS pwrs clog ilog gid γ α :
+    let ts := uint.nat tsW in
+    let clog' := clog ++ [CmdCommit ts pwrs] in
+    Forall (λ nc, (nc.1 <= length clog)%nat) ilog ->
+    valid_pwrs gid pwrs ->
+    group_histm_lbs_from_log γ gid clog' -∗
+    is_replica_idx rp γ α -∗
+    {{{ own_dbmap_in_slice pwrsS pwrs ∗
+        own_replica_replaying rp clog ilog α
+    }}}
+      Replica__applyCommit #rp #tsW (to_val pwrsS)
+    {{{ RET #(); 
+        own_dbmap_in_slice pwrsS pwrs ∗ 
+        own_replica_replaying rp clog' ilog α
+    }}}.
+  Proof.
+    iIntros (ts clog' Hvicmds Hvpwrs) "#Hhistmlb #Hidx".
+    iIntros (Φ) "!> [Hpwrs Hrp] HΦ".
+    wp_rec.
+    (* First establish that applying this commit results does not get stuck. *)
+    rewrite /group_histm_lbs_from_log.
+    destruct (apply_cmds clog') as [cm' histm' |] eqn:Happly'; last done.
+    (* Also establish connection between executing entire log vs. consistent log. *)
+    iNamed "Hrp".
+    unshelve epose proof (execute_cmds_apply_cmds clog ilog cm histm _) as Happly.
+    { by eauto 10. }
+
+    (*@ func (rp *Replica) applyCommit(ts uint64, pwrs []tulip.WriteEntry) {    @*)
+    (*@     // Query the transaction table. Note that if there's an entry for @ts in @*)
+    (*@     // @txntbl, then transaction @ts can only be committed. That's why we're not @*)
+    (*@     // even reading the value of entry.                                 @*)
+    (*@     committed := rp.terminated(ts)                                      @*)
+    (*@     if committed {                                                      @*)
+    (*@         return                                                          @*)
+    (*@     }                                                                   @*)
+    (*@                                                                         @*)
+    wp_apply (wp_Replica__terminated with "Hcm").
+    iIntros "Hcm".
+    case_bool_decide as Hterm; wp_pures.
+    { iApply "HΦ".
+      apply elem_of_dom in Hterm as [b Hb].
+      iFrame "∗ # %".
+      iPureIntro. simpl.
+      exists ptgsm.
+      rewrite merge_clog_ilog_snoc_clog; last apply Hvicmds.
+      rewrite /execute_cmds foldl_snoc /= execute_cmds_unfold Hexec /= Hb.
+      destruct b; first done.
+      by rewrite /apply_cmds foldl_snoc /= apply_cmds_unfold /apply_commit Happly Hb in Happly'.
+    }
+    apply not_elem_of_dom in Hterm.
+    rewrite /apply_cmds foldl_snoc /= apply_cmds_unfold Happly /= Hterm in Happly'.
+    case_decide as Hsafeext; last done.
+    symmetry in Happly'. inv Happly'.
+
+    (*@     rp.multiwrite(ts, pwrs)                                             @*)
+    (*@                                                                         @*)
+    wp_apply (wp_Replica__multiwrite with "Hhistmlb Hidx [$Hpwrs $Hhistm]").
+    { apply Hvpwrs. }
+    { by eapply apply_cmds_dom. }
+    { apply Hsafeext. }
+    iIntros "[Hpwrs Hhistm]".
+
+    (*@     rp.txntbl[ts] = true                                                @*)
+    (*@                                                                         @*)
+    iNamed "Hcm".
+    wp_loadField.
+    wp_apply (wp_MapInsert with "Htxntbl"); first done.
+    iIntros "Htxntbl".
+
+    (*@     // With PCR, a replica might receive a commit even if it is not prepared on @*)
+    (*@     // this replica.                                                    @*)
+    (*@     _, prepared := rp.prepm[ts]                                         @*)
+    (*@                                                                         @*)
+    iNamed "Hcpm".
+    wp_loadField.
+    wp_apply (wp_MapGet with "HprepmS").
+    iIntros (prepS prepared) "[%Hprepared HprepmS]".
+    wp_pures.
+
+    (*@     if prepared {                                                       @*)
+    (*@         rp.release(pwrs)                                                @*)
+    (*@         delete(rp.prepm, ts)                                            @*)
+    (*@     }                                                                   @*)
+    (*@ }                                                                       @*)
+    destruct prepared; wp_pures.
+    { wp_apply (wp_Replica__release with "[$Hpwrs $Hptsmsptsm]").
+      { clear -Hvpwrs. set_solver. }
+      iIntros "[Hpwrs Hptsmsptsm]".
+      wp_loadField.
+      wp_apply (wp_MapDelete with "HprepmS").
+      iIntros "HprepmS".
+      wp_pures.
+      iApply "HΦ".
+      apply map_get_true in Hprepared.
+      iDestruct (big_sepM2_delete_l with "Hprepm") as (m) "(%Hm & _ & Hprepm)".
+      { apply Hprepared. }
+      iFrame "∗ #".
+      iPureIntro. simpl.
+      exists (<[ts := true]> cm), (delete ts cpm), (delete ts ptgsm).
+      split.
+      { rewrite 2!kmap_insert. f_equal; [word | done]. }
+      split.
+      { rewrite 2!kmap_delete. f_equal; [word | done]. }
+      split.
+      { by apply map_Forall_delete. }
+      { rewrite merge_clog_ilog_snoc_clog; last apply Hvicmds.
+        symmetry in Hcpmabs.
+        pose proof (lookup_kmap_eq_Some _ _ _ _ _ _ Hcpmabs Hm) as (ts' & Hts' & Hcpmts).
+        assert (ts' = ts) as -> by word.
+        rewrite /execute_cmds foldl_snoc /= execute_cmds_unfold Hexec /= Hterm Hcpmts.
+        by case_decide.
+      }
+    }
+    iDestruct (big_sepM2_dom with "Hprepm") as %Hdomprepm.
+    iApply "HΦ".
+    iFrame "∗ # %".
+    iPureIntro. simpl.
+    exists (<[ts := true]> cm), ptgsm.
+    split.
+    { rewrite 2!kmap_insert. f_equal; [word | done]. }
+    { rewrite merge_clog_ilog_snoc_clog; last apply Hvicmds.
+      apply map_get_false in Hprepared as [Hnone _].
+      rewrite -not_elem_of_dom Hdomprepm not_elem_of_dom in Hnone.
+      symmetry in Hcpmabs.
+      pose proof (lookup_kmap_eq_None _ _ _ _ _  Hcpmabs Hnone) as Hcpmnone.
+      specialize (Hcpmnone ts).
+      unshelve epose proof (Hcpmnone _) as Hcpmts; first word.
+      rewrite /execute_cmds foldl_snoc /= execute_cmds_unfold Hexec /= Hterm Hcpmts.
+      by case_decide.
+    }
+  Qed.
+
   Theorem wp_Replica__applyCommit
     rp (tsW : u64) pwrsS pwrs cloga gid rid γ α :
     let ts := uint.nat tsW in
