src/program_proof/tulip/program/replica/replica_log.v
@@ -1,20 +1,53 @@
+From Perennial.program_proof.rsm.pure Require Import serialize.
 From Perennial.program_proof Require Import marshal_stateless_proof.
 From Perennial.program_proof.tulip.program Require Import prelude.
 From Perennial.program_proof.tulip.program.util Require Import
   encode_string encode_kvmap_from_slice.
 
+(* Copy pasted from grove_ffi_typed.v *)
+Ltac inv_undefined :=
+  match goal with
+  | [ H: relation.denote (match ?e with | _ => _ end) _ _ _ |- _ ] =>
+    destruct e; try (apply suchThat_false in H; contradiction)
+  end.
+Local Ltac solve_atomic :=
+  apply strongly_atomic_atomic, ectx_language_atomic;
+  [ apply heap_base_atomic; cbn [relation.denote base_trans]; intros * H;
+    repeat inv_undefined;
+    try solve [ apply atomically_is_val in H; auto ]
+    |apply ectxi_language_sub_redexes_are_values; intros [] **; naive_solver].
+Local Ltac solve_atomic2 :=
+  solve_atomic;
+  (* TODO(Joe): Cleanup *)
+  repeat match goal with
+    | [ H: relation.denote _ ?s1 ?s2 ?v |- _ ] => inversion_clear H
+    | _ => progress monad_inv
+    | _ => case_match
+    end; eauto.
+
 Section program.
   Context `{!heapGS Σ, !tulip_ghostG Σ}.
 
-  Theorem wp_logRead (fname : byte_string) (ts : u64) (key : byte_string) (bs : list u8) :
-    {{{ fname f↦ bs }}}
-      logRead #(LitString fname) #ts #(LitString key)
-    {{{ (bs' : list u8), RET #(); fname f↦ bs' }}}.
+  Theorem wp_logRead
+    (fname : byte_string) (lsnW tsW : u64) (key : byte_string) :
+    let lsn := uint.nat lsnW in
+    let ts := uint.nat tsW in
+    ⊢
+    {{{ True }}}
+    <<< ∀∀ bs ilog, fname f↦ bs ∗ ⌜encode_ilog ilog bs⌝ >>>
+      logRead #(LitString fname) #lsnW #tsW #(LitString key) @ ∅
+    <<< ∃∃ bs' (failed : bool),
+            if failed
+            then fname f↦ bs
+            else fname f↦ bs' ∗
+                 ⌜encode_ilog (ilog ++ [(lsn, CmdRead ts key)]) bs'⌝
+    >>>
+    {{{ RET #(); ⌜not failed⌝ }}}.
   Proof.
-    iIntros (Φ) "Hfile HΦ".
+    iIntros (lsn ts Φ) "!> _ HAU".
     wp_rec.
 
-    (*@ func logRead(fname string, ts uint64, key string) {                     @*)
+    (*@ func logRead(fname string, lsn, ts uint64, key string) {                @*)
     (*@     // Create an inconsistent log entry for reading @key at @ts.        @*)
     (*@     bs := make([]byte, 0, 32)                                           @*)
     (*@                                                                         @*)
@@ -22,7 +55,8 @@ Section program.
     iIntros (p1) "Hbs".
     rewrite uint_nat_W64_0 replicate_0.
 
-    (*@     bs1 := marshal.WriteInt(bs, CMD_READ)                               @*)
+    (*@     bs0 := marshal.WriteInt(bs, lsn)                                    @*)
+    (*@     bs1 := marshal.WriteInt(bs0, CMD_READ)                              @*)
     (*@     bs2 := marshal.WriteInt(bs1, ts)                                    @*)
     (*@     bs3 := util.EncodeString(bs2, key)                                  @*)
     (*@                                                                         @*)
@@ -30,8 +64,10 @@ Section program.
     iIntros (p2) "Hbs".
     wp_apply (wp_WriteInt with "Hbs").
     iIntros (p3) "Hbs".
-    wp_apply (wp_EncodeString with "Hbs").
+    wp_apply (wp_WriteInt with "Hbs").
     iIntros (p4) "Hbs".
+    wp_apply (wp_EncodeString with "Hbs").
+    iIntros (p5) "Hbs".
     wp_pures.
 
     (*@     grove_ffi.FileAppend(fname, bs3)                                    @*)
@@ -39,28 +75,72 @@ Section program.
     wp_rec. wp_pures.
     wp_rec. wp_pures.
     wp_rec. wp_pures.
+    wp_bind (ExternalOp _ _).
+    rewrite difference_empty_L.
+    iApply (wp_ncatomic _ _ ∅).
+    { solve_atomic2. }
     iDestruct (own_slice_to_small with "Hbs") as "Hbs".
+    rewrite -!app_assoc app_nil_l.
+    set frag := _ ++ _.
     iDestruct (own_slice_small_sz with "Hbs") as %Hszbs.
+    iMod "HAU" as (bs ilog) "[[Hfile %Henc] HAU]".
+    iModIntro.
     wp_apply (wp_FileAppendOp with "[$Hfile Hbs]").
     { apply Hszbs. }
     { iApply (own_slice_small_byte_pointsto_vals with "Hbs"). }
     iIntros (err) "[Hfile Hbs]".
+    destruct err eqn:Herr.
+    { (* Case: Write failed. *)
+      iMod ("HAU" $! bs true with "[$Hfile]") as "HΦ".
+      iModIntro.
+      wp_pures.
+      wp_apply wp_Exit. iIntros "[]".
+    }
+    (* Case: Write succeeded. *)
+    iMod ("HAU" $! _ false with "[$Hfile]") as "HΦ".
+    { iPureIntro.
+      rewrite /encode_ilog.
+      destruct Henc as (frags & Hencfrag & Hserial).
+      exists (frags ++ [frag]).
+      split.
+      { apply Forall2_app; first apply Hencfrag.
+        apply Forall2_cons_2; last by apply Forall2_nil.
+        simpl.
+        exists (u64_le (U64 0) ++ u64_le ts ++ encode_string key).
+        subst frag.
+        assert (W64 lsn = lsnW) as -> by word.
+        by assert (W64 ts = tsW) as -> by word.
+      }
+      by rewrite serialize_snoc Hserial.
+    }
+    iModIntro.
     wp_pures.
-    destruct err; wp_pures.
-    { wp_apply wp_Exit. iIntros "[]". }
-    by iApply "HΦ".
+    iApply "HΦ".
+    iFrame.
+    iPureIntro.
+    by auto.
   Qed.
 
-  Theorem wp_logValidate
-    (fname : byte_string) (ts : u64) (pwrsP : Slice.t) (pwrs : dbmap) (bs : list u8) :
-    {{{ fname f↦ bs ∗ own_dbmap_in_slice pwrsP pwrs }}}
-      logValidate #(LitString fname) #ts (to_val pwrsP) slice.nil
-    {{{ (bs' : list u8), RET #(); fname f↦ bs' ∗ own_dbmap_in_slice pwrsP pwrs }}}.
+  Theorem wp_logAcquire
+    (fname : byte_string) (lsnW tsW : u64) (pwrsP : Slice.t) (pwrs : dbmap) :
+    let lsn := uint.nat lsnW in
+    let ts := uint.nat tsW in
+    ⊢
+    {{{ own_dbmap_in_slice pwrsP pwrs }}}
+    <<< ∀∀ bs ilog, fname f↦ bs ∗ ⌜encode_ilog ilog bs⌝ >>>
+      logAcquire #(LitString fname) #lsnW #tsW (to_val pwrsP) slice.nil @ ∅
+    <<< ∃∃ bs' (failed : bool),
+            if failed
+            then fname f↦ bs
+            else fname f↦ bs' ∗
+                 ⌜encode_ilog (ilog ++ [(lsn, CmdAcquire ts pwrs ∅)]) bs'⌝
+    >>>
+    {{{ RET #(); own_dbmap_in_slice pwrsP pwrs ∗ ⌜not failed⌝ }}}.
   Proof.
-    iIntros (Φ) "[Hfile Hpwrs] HΦ".
+    iIntros (lsn ts Φ) "!> Hpwrs HAU".
     wp_rec.
 
-    (*@ func logValidate(fname string, ts uint64, pwrs []tulip.WriteEntry, ptgs []uint64) { @*)
+    (*@ func logAcquire(fname string, lsn, ts uint64, pwrs []tulip.WriteEntry, ptgs []uint64) { @*)
     (*@     // Create an inconsistent log entry for validating @ts with @pwrs and @ptgs. @*)
     (*@     bs := make([]byte, 0, 64)                                           @*)
     (*@                                                                         @*)
@@ -68,16 +148,20 @@ Section program.
     iIntros (p1) "Hbs".
     rewrite uint_nat_W64_0 replicate_0.
 
-    (*@     bs1 := marshal.WriteInt(bs, CMD_VALIDATE)                           @*)
+    (*@     bs0 := marshal.WriteInt(bs, lsn)                                    @*)
+    (*@     bs1 := marshal.WriteInt(bs0, CMD_ACQUIRE)                           @*)
     (*@     bs2 := marshal.WriteInt(bs1, ts)                                    @*)
     (*@     bs3 := util.EncodeKVMapFromSlice(bs2, pwrs)                         @*)
+    (*@     // TODO: encode ptgs                                                @*)
     (*@                                                                         @*)
     wp_apply (wp_WriteInt with "Hbs").
     iIntros (p2) "Hbs".
     wp_apply (wp_WriteInt with "Hbs").
     iIntros (p3) "Hbs".
+    wp_apply (wp_WriteInt with "Hbs").
+    iIntros (p4) "Hbs".
     wp_apply (wp_EncodeKVMapFromSlice with "[$Hbs $Hpwrs]").
-    iIntros (p4 mdata) "[Hbs [Hpwrs %Hmdata]]".
+    iIntros (p5 mdata) "[Hbs [Hpwrs %Hmdata]]".
     wp_pures.
 
     (*@     grove_ffi.FileAppend(fname, bs3)                                    @*)
@@ -85,75 +169,199 @@ Section program.
     wp_rec. wp_pures.
     wp_rec. wp_pures.
     wp_rec. wp_pures.
+    wp_bind (ExternalOp _ _).
+    rewrite difference_empty_L.
+    iApply (wp_ncatomic _ _ ∅).
+    { solve_atomic2. }
     iDestruct (own_slice_to_small with "Hbs") as "Hbs".
+    rewrite -!app_assoc app_nil_l.
+    set frag := _ ++ _.
     iDestruct (own_slice_small_sz with "Hbs") as %Hszbs.
+    iMod "HAU" as (bs ilog) "[[Hfile %Henc] HAU]".
+    iModIntro.
     wp_apply (wp_FileAppendOp with "[$Hfile Hbs]").
     { apply Hszbs. }
     { iApply (own_slice_small_byte_pointsto_vals with "Hbs"). }
     iIntros (err) "[Hfile Hbs]".
+    destruct err eqn:Herr.
+    { (* Case: Write failed. *)
+      iMod ("HAU" $! bs true with "[$Hfile]") as "HΦ".
+      iModIntro.
+      wp_pures.
+      wp_apply wp_Exit. iIntros "[]".
+    }
+    (* Case: Write succeeded. *)
+    iMod ("HAU" $! _ false with "[$Hfile]") as "HΦ".
+    { iPureIntro.
+      rewrite /encode_ilog.
+      destruct Henc as (frags & Hencfrag & Hserial).
+      exists (frags ++ [frag]).
+      split.
+      { apply Forall2_app; first apply Hencfrag.
+        apply Forall2_cons_2; last by apply Forall2_nil.
+        simpl.
+        exists (u64_le (U64 1) ++ u64_le ts ++ mdata).
+        subst frag.
+        assert (W64 lsn = lsnW) as -> by word.
+        assert (W64 ts = tsW) as -> by word.
+        split; first done.
+        by exists mdata.
+      }
+      by rewrite serialize_snoc Hserial.
+    }
+    iModIntro.
     wp_pures.
-    destruct err; wp_pures.
-    { wp_apply wp_Exit. iIntros "[]". }
     iApply "HΦ".
-    by iFrame.
+    iFrame.
+    iPureIntro.
+    by auto.
   Qed.
 
   Theorem wp_logFastPrepare
-    (fname : byte_string) (ts : u64) (pwrsP : Slice.t) (pwrs : dbmap) (bs : list u8) :
-    {{{ fname f↦ bs ∗ own_dbmap_in_slice pwrsP pwrs }}}
-      logFastPrepare #(LitString fname) #ts (to_val pwrsP) slice.nil
-    {{{ (bs' : list u8), RET #(); fname f↦ bs' ∗ own_dbmap_in_slice pwrsP pwrs }}}.
+    (fname : byte_string) (lsnW tsW : u64) (pwrsP : Slice.t) (pwrs : dbmap) :
+    let lsn := uint.nat lsnW in
+    let ts := uint.nat tsW in
+    let icmds := [(lsn, CmdAcquire ts pwrs ∅); (lsn, CmdAccept ts O true)] in
+    ⊢
+    {{{ own_dbmap_in_slice pwrsP pwrs }}}
+    <<< ∀∀ bs ilog, fname f↦ bs ∗ ⌜encode_ilog ilog bs⌝ >>>
+      logFastPrepare #(LitString fname) #lsnW #tsW (to_val pwrsP) slice.nil @ ∅
+    <<< ∃∃ bs' (failed : bool),
+            if failed
+            then fname f↦ bs
+            else fname f↦ bs' ∗
+                 ⌜encode_ilog (ilog ++ icmds) bs'⌝
+    >>>
+    {{{ RET #(); own_dbmap_in_slice pwrsP pwrs ∗ ⌜not failed⌝ }}}.
   Proof.
-    iIntros (Φ) "[Hfile Hpwrs] HΦ".
+    iIntros (lsn ts icmds Φ) "!> Hpwrs HAU".
     wp_rec.
 
-    (*@ func logFastPrepare(fname string, ts uint64, pwrs []tulip.WriteEntry, ptgs []uint64) { @*)
+    (*@ func logFastPrepare(fname string, lsn, ts uint64, pwrs []tulip.WriteEntry, ptgs []uint64) { @*)
     (*@     // Create an inconsistent log entry for fast preparing @ts.         @*)
-    (*@     bs := make([]byte, 0, 64)                                           @*)
+    (*@     bs := make([]byte, 0, 128)                                          @*)
     (*@                                                                         @*)
     wp_apply wp_NewSliceWithCap; first word.
     iIntros (p1) "Hbs".
     rewrite uint_nat_W64_0 replicate_0.
 
-    (*@     bs1 := marshal.WriteInt(bs, CMD_FAST_PREPARE)                       @*)
+    (*@     bs0 := marshal.WriteInt(bs, lsn)                                    @*)
+    (*@     bs1 := marshal.WriteInt(bs0, CMD_ACQUIRE)                           @*)
     (*@     bs2 := marshal.WriteInt(bs1, ts)                                    @*)
     (*@     bs3 := util.EncodeKVMapFromSlice(bs2, pwrs)                         @*)
+    (*@     // TODO: encode ptgs                                                @*)
+    (*@     bs4 := marshal.WriteInt(bs3, lsn)                                   @*)
+    (*@     bs5 := marshal.WriteInt(bs4, CMD_ACCEPT)                            @*)
+    (*@     bs6 := marshal.WriteInt(bs5, ts)                                    @*)
+    (*@     bs7 := marshal.WriteInt(bs6, 0)                                     @*)
+    (*@     bs8 := marshal.WriteBool(bs7, true)                                 @*)
     (*@                                                                         @*)
     wp_apply (wp_WriteInt with "Hbs").
     iIntros (p2) "Hbs".
     wp_apply (wp_WriteInt with "Hbs").
     iIntros (p3) "Hbs".
+    wp_apply (wp_WriteInt with "Hbs").
+    iIntros (p4) "Hbs".
     wp_apply (wp_EncodeKVMapFromSlice with "[$Hbs $Hpwrs]").
-    iIntros (p4 mdata) "[Hbs [Hpwrs %Hmdata]]".
+    iIntros (p5 mdata) "[Hbs [Hpwrs %Hmdata]]".
+    wp_pures.
+    wp_apply (wp_WriteInt with "Hbs").
+    iIntros (p6) "Hbs".
+    wp_apply (wp_WriteInt with "Hbs").
+    iIntros (p7) "Hbs".
+    wp_apply (wp_WriteInt with "Hbs").
+    iIntros (p8) "Hbs".
+    wp_apply (wp_WriteInt with "Hbs").
+    iIntros (p9) "Hbs".
+    wp_apply (wp_WriteBool with "Hbs").
+    iIntros (p10) "Hbs".
     wp_pures.
 
-    (*@     grove_ffi.FileAppend(fname, bs3)                                    @*)
+    (*@     grove_ffi.FileAppend(fname, bs8)                                    @*)
     (*@ }                                                                       @*)
     wp_rec. wp_pures.
     wp_rec. wp_pures.
     wp_rec. wp_pures.
+    wp_bind (ExternalOp _ _).
+    rewrite difference_empty_L.
+    iApply (wp_ncatomic _ _ ∅).
+    { solve_atomic2. }
     iDestruct (own_slice_to_small with "Hbs") as "Hbs".
+    rewrite -4!app_assoc app_nil_l.
+    rewrite -(app_assoc _ _ mdata).
+    rewrite -(app_assoc _ _ (u64_le tsW ++ mdata)).
+    set fragacq := _ ++ u64_le (W64 1) ++ _.
+    set fragacp := _ ++ u64_le (W64 3) ++ _.
     iDestruct (own_slice_small_sz with "Hbs") as %Hszbs.
+    iMod "HAU" as (bs ilog) "[[Hfile %Henc] HAU]".
+    iModIntro.
     wp_apply (wp_FileAppendOp with "[$Hfile Hbs]").
     { apply Hszbs. }
     { iApply (own_slice_small_byte_pointsto_vals with "Hbs"). }
     iIntros (err) "[Hfile Hbs]".
+    destruct err eqn:Herr.
+    { (* Case: Write failed. *)
+      iMod ("HAU" $! bs true with "[$Hfile]") as "HΦ".
+      iModIntro.
+      wp_pures.
+      wp_apply wp_Exit. iIntros "[]".
+    }
+    (* Case: Write succeeded. *)
+    iMod ("HAU" $! _ false with "[$Hfile]") as "HΦ".
+    { iPureIntro.
+      rewrite /encode_ilog.
+      destruct Henc as (frags & Hencfrag & Hserial).
+      exists (frags ++ [fragacq; fragacp]).
+      split.
+      { apply Forall2_app; first apply Hencfrag.
+        apply Forall2_cons_2.
+        { simpl.
+          exists (u64_le (U64 1) ++ u64_le ts ++ mdata).
+          subst fragacq.
+          assert (W64 lsn = lsnW) as -> by word.
+          assert (W64 ts = tsW) as -> by word.
+          split; first done.
+          by exists mdata.
+        }
+        apply Forall2_cons_2; last by apply Forall2_nil.
+        simpl.
+        exists (u64_le (U64 3) ++ u64_le ts ++ u64_le (U64 O) ++ [U8 1]).
+        subst fragacp.
+        assert (W64 lsn = lsnW) as -> by word.
+        assert (W64 ts = tsW) as -> by word.
+        done.
+      }
+      by rewrite serialize_app Hserial.
+    }
+    iModIntro.
     wp_pures.
-    destruct err; wp_pures.
-    { wp_apply wp_Exit. iIntros "[]". }
     iApply "HΦ".
-    by iFrame.
+    iFrame.
+    iPureIntro.
+    by auto.
   Qed.
 
-  Theorem wp_logAccept (fname : byte_string) (ts : u64) (rank : u64) (dec : bool) (bs : list u8) :
-    {{{ fname f↦ bs }}}
-      logAccept #(LitString fname) #ts #rank #dec
-    {{{ (bs' : list u8), RET #(); fname f↦ bs' }}}.
+  Theorem wp_logAccept
+    (fname : byte_string) (lsnW tsW rankW : u64) (dec : bool) :
+    let lsn := uint.nat lsnW in
+    let ts := uint.nat tsW in
+    let rank := uint.nat rankW in
+    ⊢
+    {{{ True }}}
+    <<< ∀∀ bs ilog, fname f↦ bs ∗ ⌜encode_ilog ilog bs⌝ >>>
+      logAccept #(LitString fname) #lsnW #tsW #rankW #dec @ ∅
+    <<< ∃∃ bs' (failed : bool),
+            if failed
+            then fname f↦ bs
+            else fname f↦ bs' ∗
+                 ⌜encode_ilog (ilog ++ [(lsn, CmdAccept ts rank dec)]) bs'⌝
+    >>>
+    {{{ RET #(); ⌜not failed⌝ }}}.
   Proof.
-    iIntros (Φ) "Hfile HΦ".
+    iIntros (lsn ts rank Φ) "!> _ HAU".
     wp_rec.
 
-    (*@ func logAccept(fname string, ts uint64, rank uint64, dec bool) {        @*)
+    (*@ func logAccept(fname string, lsn, ts uint64, rank uint64, dec bool) {   @*)
     (*@     // Create an inconsistent log entry for accepting prepare decision @dec for @*)
     (*@     // @ts in @rank.                                                    @*)
     (*@     bs := make([]byte, 0, 32)                                           @*)
@@ -162,7 +370,8 @@ Section program.
     iIntros (p1) "Hbs".
     rewrite uint_nat_W64_0 replicate_0.
 
-    (*@     bs1 := marshal.WriteInt(bs, CMD_ACCEPT)                             @*)
+    (*@     bs0 := marshal.WriteInt(bs, lsn)                                    @*)
+    (*@     bs1 := marshal.WriteInt(bs0, CMD_ACCEPT)                            @*)
     (*@     bs2 := marshal.WriteInt(bs1, ts)                                    @*)
     (*@     bs3 := marshal.WriteInt(bs2, rank)                                  @*)
     (*@     bs4 := marshal.WriteBool(bs3, dec)                                  @*)
@@ -173,8 +382,10 @@ Section program.
     iIntros (p3) "Hbs".
     wp_apply (wp_WriteInt with "Hbs").
     iIntros (p4) "Hbs".
-    wp_apply (wp_WriteBool with "Hbs").
+    wp_apply (wp_WriteInt with "Hbs").
     iIntros (p5) "Hbs".
+    wp_apply (wp_WriteBool with "Hbs").
+    iIntros (p6) "Hbs".
     wp_pures.
 
     (*@     grove_ffi.FileAppend(fname, bs4)                                    @*)
@@ -182,17 +393,51 @@ Section program.
     wp_rec. wp_pures.
     wp_rec. wp_pures.
     wp_rec. wp_pures.
+    wp_bind (ExternalOp _ _).
+    rewrite difference_empty_L.
+    iApply (wp_ncatomic _ _ ∅).
+    { solve_atomic2. }
     iDestruct (own_slice_to_small with "Hbs") as "Hbs".
+    rewrite -!app_assoc app_nil_l.
+    set frag := _ ++ _.
     iDestruct (own_slice_small_sz with "Hbs") as %Hszbs.
+    iMod "HAU" as (bs ilog) "[[Hfile %Henc] HAU]".
+    iModIntro.
     wp_apply (wp_FileAppendOp with "[$Hfile Hbs]").
     { apply Hszbs. }
     { iApply (own_slice_small_byte_pointsto_vals with "Hbs"). }
     iIntros (err) "[Hfile Hbs]".
+    destruct err eqn:Herr.
+    { (* Case: Write failed. *)
+      iMod ("HAU" $! bs true with "[$Hfile]") as "HΦ".
+      iModIntro.
+      wp_pures.
+      wp_apply wp_Exit. iIntros "[]".
+    }
+    (* Case: Write succeeded. *)
+    iMod ("HAU" $! _ false with "[$Hfile]") as "HΦ".
+    { iPureIntro.
+      rewrite /encode_ilog.
+      destruct Henc as (frags & Hencfrag & Hserial).
+      exists (frags ++ [frag]).
+      split.
+      { apply Forall2_app; first apply Hencfrag.
+        apply Forall2_cons_2; last by apply Forall2_nil.
+        simpl.
+        exists (u64_le (U64 3) ++ u64_le ts ++ u64_le rank ++ [if dec then W8 1 else W8 0]).
+        subst frag.
+        assert (W64 lsn = lsnW) as -> by word.
+        assert (W64 ts = tsW) as -> by word.
+        by assert (W64 rank = rankW) as -> by word.
+      }
+      by rewrite serialize_snoc Hserial.
+    }
+    iModIntro.
     wp_pures.
-    destruct err; wp_pures.
-    { wp_apply wp_Exit. iIntros "[]". }
     iApply "HΦ".
-    by iFrame.
+    iFrame.
+    iPureIntro.
+    by auto.
   Qed.
 
 End program.
