src/program_proof/tulip/program/replica/replica_prepare.v
@@ -32,7 +32,7 @@ Section program.
     wp_loadField.
     wp_apply (wp_Mutex__Lock with "Hlock").
     iIntros "[Hlocked Hrp]".
-    wp_apply (wp_Replica__tryAccept with "Hppsl Hinv Hrp").
+    wp_apply (wp_Replica__tryAccept with "Hppsl Hinv Hinvfile Hrp").
     { apply Hgid. }
     { apply Hrid. }
     { apply Hranknz. }
