src/program_proof/tulip/program/replica/replica_resume.v
@@ -1,0 +1,711 @@
+From Perennial.program_proof.rsm.pure Require Import serialize.
+From Perennial.program_proof.tulip.program Require Import prelude.
+From Perennial.program_proof.tulip.program.replica Require Import  replica_repr.
+From Perennial.program_proof Require Import marshal_stateless_proof.
+From Perennial.program_proof.tulip.program.util Require Import
+  decode_string.
+From Goose.github_com.mit_pdos.tulip Require Import replica.
+From Perennial.program_proof.tulip.paxos Require Import prelude.
+
+(* for replay *)
+From Perennial.program_proof.tulip.program.util Require Import
+  decode_string decode_kvmap_into_slice.
+From Perennial.program_proof.tulip.program.replica Require Import
+  replica_apply replica_bump_key replica_acquire replica_memorize
+  replica_advance replica_accept.
+From Perennial.program_proof.tulip.program.txnlog Require Import txnlog.
+From Perennial.program_proof.tulip.invariance Require Import learn.
+
+Opaque u64_le.
+
+(* Copy pasted from grove_ffi_typed.v *)
+Ltac inv_undefined :=
+  match goal with
+  | [ H: relation.denote (match ?e with | _ => _ end) _ _ _ |- _ ] =>
+    destruct e; try (apply suchThat_false in H; contradiction)
+  end.
+Local Ltac solve_atomic :=
+  apply strongly_atomic_atomic, ectx_language_atomic;
+  [ apply heap_base_atomic; cbn [relation.denote base_trans]; intros * H;
+    repeat inv_undefined;
+    try solve [ apply atomically_is_val in H; auto ]
+    |apply ectxi_language_sub_redexes_are_values; intros [] **; naive_solver].
+Local Ltac solve_atomic2 :=
+  solve_atomic;
+  (* TODO(Joe): Cleanup *)
+  repeat match goal with
+    | [ H: relation.denote _ ?s1 ?s2 ?v |- _ ] => inversion_clear H
+    | _ => progress monad_inv
+    | _ => case_match
+    end; eauto.
+
+Section program.
+  Context `{!heapGS Σ, !tulip_ghostG Σ, !paxos_ghostG Σ}.
+
+  Theorem wp_Replica__replay (rp : loc) (lsnW : u64) ilog gid γ α :
+    let lsn := uint.nat lsnW in
+    gid ∈ gids_all ->
+    Forall (λ nc : nat * icommand, (nc.1 <= lsn)%nat) ilog ->
+    know_tulip_inv γ -∗
+    is_replica_idx rp γ α -∗
+    is_replica_txnlog rp gid γ -∗
+    {{{ own_replica_replaying_in_lsn rp lsn ilog gid γ α }}}
+      Replica__replay #rp #lsnW
+    {{{ RET #(); own_replica_replaying_in_lsn rp (S lsn) ilog gid γ α }}}.
+  Proof.
+    iIntros (lsn Hgid Hlsn) "#Hinv #Hidx #Htxnlog".
+    iIntros (Φ) "!> Hrp HΦ".
+    wp_rec.
+
+    (*@ func (rp *Replica) replay(lsn uint64) {                                 @*)
+    (*@     var cmd txnlog.Cmd                                                  @*)
+    (*@     var ok bool = false                                                 @*)
+    (*@                                                                         @*)
+    wp_apply wp_ref_of_zero; first done.
+    iIntros (cmdP) "HcmdP".
+    wp_apply wp_ref_to; first by auto.
+    iIntros (okP) "HokP".
+
+    (*@     for !ok {                                                           @*)
+    (*@         cmd, ok = rp.txnlog.Lookup(lsn)                                 @*)
+    (*@     }                                                                   @*)
+    (*@                                                                         @*)
+    iNamed "Hrp".
+    set P := (λ cont : bool,
+                ∃ (pwrsS : Slice.t) (cmd : ccommand) (ok : bool),
+                  "HcmdP"  ∷ cmdP ↦[struct.t Cmd] (ccommand_to_val pwrsS cmd) ∗
+                  "HokP"   ∷ okP ↦[boolT] #ok ∗
+                  "Hpwrs"  ∷ (if ok then own_pwrs_slice pwrsS cmd else True) ∗
+                  "#Hlb"   ∷ (if ok then is_txn_log_lb γ gid (clog ++ [cmd]) else True) ∗
+                  "%Hcont" ∷ ⌜if cont then True else ok⌝)%I.
+    wp_apply (wp_forBreak_cond P with "[] [HcmdP HokP]"); last first; first 1 last.
+    { iFrame.
+      iExists Slice.nil, (CmdAbort O).
+      rewrite /= Nat2Z.inj_0.
+      by iFrame.
+    }
+    { clear Φ.
+      iIntros (Φ) "!> HP HΦ".
+      iNamed "HP".
+      wp_load.
+      destruct ok; wp_pures.
+      { (* Loop exit. *)
+        iApply "HΦ".
+        by iFrame "HcmdP HokP Hpwrs Hlb".
+      }
+      iNamed "Htxnlog".
+      wp_loadField.
+      wp_apply (wp_TxnLog__Lookup with "Htxnlog").
+      iDestruct "Hinv" as (proph) "Hinv".
+      iInv "Hinv" as "> HinvO" "HinvC".
+      iApply ncfupd_mask_intro; first set_solver.
+      iIntros "Hmask".
+      iNamed "HinvO".
+      iDestruct (big_sepS_elem_of_acc with "Hgroups") as "[Hgroup HgroupsC]".
+      { apply Hgid. }
+      iNamed "Hgroup".
+      iDestruct (txn_log_witness with "Hlog") as "#Hloglb".
+      (* Pass the consensus resources to the paxos library. *)
+      iFrame "Hlog Hcpool".
+      (* Get back the updated resources. *)
+      iIntros (log') "[[Hlog Hcpool] %Hincl]".
+      iDestruct (txn_log_witness with "Hlog") as "#Hloglb'".
+      iDestruct (txn_log_prefix with "Hlog Hloglb") as %Hprefix.
+      destruct Hprefix as [l Hprefix].
+      iDestruct (txn_log_prefix with "Hlog Hcloglb") as %Hprefixc.
+      iAssert (group_inv_no_log_with_cpool γ gid log cpool)%I with "[$Hgroup $Hcpool]" as "Hgroup".
+      iMod (group_inv_learn with "Htxnsys Hkeys Hgroup") as "(Htxnsys & Hkeys & Hgroup)".
+      { by rewrite Hprefix in Hincl. }
+      rewrite -Hprefix.
+      iDestruct (group_inv_merge_log_hide_cpool with "Hlog Hgroup") as "Hgroup".
+      iDestruct ("HgroupsC" with "Hgroup") as "Hgroups".
+      iMod "Hmask" as "_".
+      iMod ("HinvC" with "[$Htxnsys $Hkeys $Hgroups $Hrgs]") as "_".
+      iModIntro.
+      iClear "Hpwrs".
+      iIntros (c ok pwrsP) "[Hpwrs %Hc]".
+      wp_pures.
+      wp_apply (wp_StoreAt with "HcmdP").
+      { destruct c; simpl; by auto 10. }
+      iIntros "HcmdP".
+      wp_store.
+      iApply "HΦ".
+      iFrame.
+      destruct ok; last done.
+      iDestruct (txn_log_lb_weaken (clog ++ [c]) with "Hloglb'") as "Hcloglb'".
+      { destruct Hprefixc as [lc Hprefixc].
+        rewrite Hprefixc.
+        apply prefix_app, prefix_singleton.
+        rewrite Hprefixc lookup_app_r in Hc; last first.
+        { clear -Hlenclog. lia. }
+        by rewrite Hlenclog Nat.sub_diag in Hc.
+      }
+      by iFrame "#".
+    }
+
+    (*@     rp.apply(cmd)                                                       @*)
+    (*@ }                                                                       @*)
+    iNamed 1.
+    destruct ok; last done.
+    iAssert (|={⊤}=>
+               group_histm_lbs_from_log γ gid (clog ++ [cmd]) ∗
+               ⌜valid_ccommand gid cmd⌝)%I as "> [#Hhistm %Hvcmd]".
+    { iDestruct "Hinv" as (proph) "Hinv".
+      iInv "Hinv" as "> HinvO" "HinvC".
+      iNamed "HinvO".
+      iDestruct (big_sepS_elem_of_acc with "Hgroups") as "[Hgroup HgroupsC]".
+      { apply Hgid. }
+      iDestruct (group_inv_impl_valid_ccommand_log with "Hlb Hgroup")
+        as %Hvcmds.
+      apply Forall_app in Hvcmds as [_ Hvcmd].
+      rewrite Forall_singleton in Hvcmd.
+      iDestruct (group_inv_witness_group_histm_lbs_from_log with "Hlb Hgroup")
+        as "#Hhistm".
+      iDestruct ("HgroupsC" with "Hgroup") as "Hgroups".
+      iMod ("HinvC" with "[$Htxnsys $Hkeys $Hgroups $Hrgs]") as "_".
+      iModIntro.
+      by iFrame "Hhistm".
+    }
+    wp_load.
+    wp_apply (wp_Replica__apply__replaying with "[] Hidx [$Hrp $Hpwrs]").
+    { rewrite Hlenclog. apply Hlsn. }
+    { apply Hvcmd. }
+    { iFrame "Hhistm". }
+    iIntros "[Hpwrs Hrp]".
+    wp_pures.
+    iApply "HΦ".
+    iFrame "∗ #".
+    iPureIntro.
+    rewrite length_app /= Hlenclog.
+    lia.
+  Qed.
+
+  Theorem wp_Replica__replayBetween
+    (rp : loc) (lsnxW : u64) (lsnyW : u64) ilog gid γ α :
+    let lsnx := uint.nat lsnxW in
+    let lsny := uint.nat lsnyW in
+    gid ∈ gids_all ->
+    Forall (λ nc : nat * icommand, (nc.1 <= lsnx)%nat) ilog ->
+    (lsnx ≤ lsny)%nat ->
+    know_tulip_inv γ -∗
+    is_replica_idx rp γ α -∗
+    is_replica_txnlog rp gid γ -∗
+    {{{ own_replica_replaying_in_lsn rp lsnx ilog gid γ α }}}
+      Replica__replayBetween #rp #lsnxW #lsnyW
+    {{{ RET #(); own_replica_replaying_in_lsn rp lsny ilog gid γ α }}}.
+  Proof.
+    iIntros (lsnx lsny Hgid Hlsnx Hxy) "#Hinv #Hidx #Htxnlog".
+    iIntros (Φ) "!> Hrp HΦ".
+    wp_rec.
+
+    (*@ func (rp *Replica) replayBetween(lsnx, lsny uint64) {                   @*)
+    (*@     for lsn := lsnx; lsn < lsny; lsn++ {                                @*)
+    (*@         rp.replay(lsn)                                                  @*)
+    (*@     }                                                                   @*)
+    (*@ }                                                                       @*)
+    wp_apply wp_ref_to; first by auto.
+    iIntros (lsnP) "HlsnP".
+    set P := (λ lsnW : u64,
+                "Hrp"  ∷ own_replica_replaying_in_lsn rp (uint.nat lsnW) ilog gid γ α ∗
+                "%Hge" ∷ ⌜(lsnx ≤ uint.nat lsnW)%nat⌝)%I.
+    wp_pures.
+    wp_apply (wp_forUpto P with "[] [$Hrp $HlsnP]").
+    { clear -Hxy. word. }
+    { clear Φ.
+      iIntros (lsnW Φ) "!> (HP & HlsnP & %Hbound) HΦ".
+      wp_load.
+      iNamed "HP".
+      wp_apply (wp_Replica__replay with "Hinv Hidx Htxnlog Hrp").
+      { apply Hgid. }
+      { apply (Forall_impl _ _ _ Hlsnx). clear -Hge. word. }
+      iIntros "Hrp".
+      wp_pures.
+      iApply "HΦ".
+      subst P. simpl.
+      rewrite uint_nat_word_add_S; last first.
+      { clear -Hbound. word. }
+      iFrame.
+      iPureIntro. clear -Hge. word.
+    }
+    { done. }
+    iIntros "[HP HlsnP]".
+    iNamed "HP".
+    wp_pures.
+    iApply "HΦ".
+    by iFrame.
+  Qed.
+
+  Theorem wp_Replica__resume
+    (rp : loc) (clog : dblog) (ilog : list (nat * icommand)) gid rid γ α :
+    let dst := ReplicaDurable clog ilog in
+    gid ∈ gids_all ->
+    rid ∈ rids_all ->
+    know_tulip_inv γ -∗
+    know_replica_file_inv γ gid rid -∗
+    is_replica_fname rp gid rid γ -∗
+    is_replica_idx rp γ α -∗
+    is_replica_txnlog rp gid γ -∗
+    {{{ own_replica_replaying rp [] [] α ∗
+        own_replica_lsna rp O ∗
+        own_crash_ex rpcrashNS (own_replica_durable γ gid rid) dst
+    }}}
+      Replica__resume #rp
+    {{{ RET #();
+        own_replica_replaying rp clog ilog α ∗
+        own_replica_lsna rp (length clog) ∗
+        own_crash_ex rpcrashNS (own_replica_durable γ gid rid) dst
+    }}}.
+  Proof.
+    iIntros (dst Hgid Hrid) "#Hinv #Hinvfile #Hfname #Hidx #Htxnlog".
+    iIntros (Φ) "!> (Hrp & Hlsna & Hdurable) HΦ".
+    wp_rec.
+
+    (*@ func (rp *Replica) resume() {                                           @*)
+    (*@     // Set the starting LSN to 0.                                       @*)
+    (*@     var lsnx uint64 = 0                                                 @*)
+    (*@                                                                         @*)
+    wp_apply wp_ref_to; first by auto.
+    iIntros (lsnxP) "HlsnxP".
+
+    (*@     // Read the inconsistent log.                                       @*)
+    (*@     var data = grove_ffi.FileRead(rp.fname)                             @*)
+    (*@                                                                         @*)
+    iNamed "Hfname".
+    wp_loadField.
+    wp_pures.
+    wp_rec. wp_pures.
+    wp_bind (ExternalOp _ _).
+    iApply (wp_ncatomic _ _ ∅).
+    { solve_atomic2. }
+    iMod (own_crash_ex_open with "Hdurable") as "[> Hdurable HdurableC]".
+    { solve_ndisj. }
+    iNamed "Hdurable".
+    (* Open the file invariant to obtain (1) the file points-to, (2) encoding
+    relation between the file content and the inconsistent log. *)
+    iInv "Hinvfile" as "> HinvfileO" "HinvfileC".
+    iNamed "HinvfileO".
+    iDestruct (replica_ilog_fname_agree with "Hfname Hilogfname") as %->.
+    iDestruct (replica_ilog_agree with "Hilog Hilogfileinv") as %->.
+    iApply ncfupd_mask_intro; first solve_ndisj.
+    iIntros "Hmask".
+    wp_apply (wp_FileReadOp with "Hfile").
+    iIntros (err p len) "[Hfile HdataP]".
+    iMod "Hmask" as "_".
+    iMod ("HinvfileC" with "[Hilogfileinv Hfile]") as "_".
+    { iFrame "∗ # %". }
+    iMod ("HdurableC" $! dst with "[$Hclog $Hilog]") as "Hdurable".
+    iModIntro.
+    destruct err; wp_pures.
+    { wp_apply wp_Exit. iIntros "[]". }
+    iDestruct "HdataP" as "[%Hlen HdataP]".
+    set dataP := Slice.mk p len len.
+    iDestruct (pointsto_vals_own_slice_small_byte dataP with "HdataP") as "Hdata".
+    { done. }
+    { done. }
+    wp_apply wp_ref_to.
+    { apply (slice_val_ty dataP). }
+    iIntros (dataPP) "HdataPP".
+    wp_pures.
+
+    iAssert (|NC={⊤}=>
+               (own_crash_ex rpcrashNS (own_replica_durable γ gid rid) dst ∗
+                is_txn_log_lb γ gid clog ∗
+                ⌜ilog_lsn_sorted ilog⌝ ∗
+                ⌜eq_lsn_last_ilog (length clog) ilog⌝))%I
+      with "[Hdurable]" as "> (Hdurable & #Hloglb & %Hsorted & %Heqlast)".
+    { iMod (own_crash_ex_open with "Hdurable") as "[> Hdurable HdurableC]".
+      { solve_ndisj. }
+      iNamedSuffix "Hdurable" "X".
+      iDestruct "Hinv" as (proph) "Hinv".
+      iInv "Hinv" as "> HinvO" "HinvC".
+      iNamed "HinvO".
+      iDestruct (big_sepS_elem_of_acc with "Hrgs") as "[Hrg HrgsC]".
+      { apply Hgid. }
+      iDestruct (big_sepS_elem_of_acc with "Hrg") as "[Hrp HrgC]".
+      { apply Hrid. }
+      do 2 iNamed "Hrp".
+      iDestruct (replica_clog_agree with "HclogX Hclog") as %->.
+      iDestruct (replica_ilog_agree with "HilogX Hilog") as %->.
+      iDestruct ("HrgC" with "[$Hvtss $Hclog $Hilog $Hkvdm $Hbm $Hbackup]") as "Hrg".
+      { by iFrame "# %". }
+      iDestruct ("HrgsC" with "Hrg") as "Hrgs".
+      iMod ("HinvC" with "[$Htxnsys $Hkeys $Hgroups $Hrgs]") as "_".
+      iMod ("HdurableC" $! dst with "[$HclogX $HilogX]") as "Hdurable".
+      by iFrame "∗ # %".
+    }
+
+    (*@     for 0 < uint64(len(data)) {                                         @*)
+    (*@                                                                         @*)
+    set P := (λ cont : bool,
+                ∃ (q : Slice.t) (remaining : list w8) (ilogrbs : list byte_string)
+                  (iloga ilogr : list (nat * icommand)) (lsnx : u64),
+                  "HdataPP"  ∷ dataPP ↦[slice.T byteT] q ∗
+                  "Hdata"    ∷ own_slice_small q byteT (DfracOwn 1) remaining ∗
+                  "HlsnxP"   ∷ lsnxP ↦[uint64T] #lsnx ∗
+                  "Hrp"      ∷ own_replica_replaying_in_lsn rp (uint.nat lsnx) iloga gid γ α ∗
+                  "%Hlsnx"   ∷ ⌜eq_lsn_last_ilog (uint.nat lsnx) iloga⌝ ∗
+                  "%Hlelsnx" ∷ ⌜Forall (λ nc : nat * icommand, (nc.1 <= uint.nat lsnx)%nat) iloga⌝ ∗
+                  "%Hilogar" ∷ ⌜ilog = iloga ++ ilogr⌝ ∗
+                  "%Hserial" ∷ ⌜serialize id ilogrbs = remaining⌝ ∗
+                  "%Hilogr"  ∷ ⌜encode_ilog_frag ilogr ilogrbs⌝ ∗
+                  "%Hcont"   ∷ ⌜if cont then True else length remaining = O⌝)%I.
+    wp_apply (wp_forBreak_cond P with "[] [$Hdata $HdataPP $HlsnxP $Hrp]");
+      last first; first 1 last.
+    { iDestruct (txn_log_lb_weaken [] with "Hloglb") as "Hloglbnil".
+      { apply prefix_nil. }
+      iFrame "Hloglbnil".
+      iPureIntro. simpl.
+      destruct Hencilog as (ilogbytes & Hencfrag & Hserial).
+      by exists ilogbytes, ilog.
+    }
+    { clear Φ.
+      iIntros (Φ) "!> HP HΦ".
+      iNamed "HP".
+      wp_load.
+      wp_apply wp_slice_len.
+      wp_pures.
+      iDestruct (own_slice_small_sz with "Hdata") as %Hlenr.
+      case_bool_decide as Hbound; wp_pures; last first.
+      { iApply "HΦ".
+        iFrame "∗ # %".
+        iPureIntro.
+        clear -Hbound Hlenr. word.
+      }
+      assert (Hrem : length remaining ≠ O).
+      { clear -Hbound Hlenr. word. }
+      destruct ilogr as [| cmd ilogr'] eqn:Hilogreq.
+      { apply length_not_nil_inv in Hrem.
+        rewrite /encode_ilog_frag in Hilogr.
+        apply Forall2_nil_inv_l in Hilogr. subst ilogrbs.
+        by rewrite serialize_nil in Hserial.
+      }
+      apply Forall2_cons_inv_l in Hilogr as (cmdbs & ilogrbs' & Hcmd & Hilogr & ->).
+      destruct Hcmd as (cmddata & Hdata & Henc).
+      rewrite serialize_cons /= Hdata -app_assoc in Hserial.
+      rewrite -Hserial.
+      wp_load.
+
+      (*@         lsny, bs1 := marshal.ReadInt(data)                              @*)
+      (*@                                                                         @*)
+      wp_apply (wp_ReadInt with "Hdata").
+      iIntros (q') "Hdata".
+
+      (*@         rp.replayBetween(lsnx, lsny)                                    @*)
+      (*@                                                                         @*)
+      assert (Hinilog : cmd ∈ ilog).
+      { clear -Hilogar. set_solver. }
+      rewrite Forall_forall in Hvilog.
+      specialize (Hvilog _ Hinilog).
+      destruct Hvilog as [Hvlsn Hvicmd].
+      wp_load.
+      assert (Hlsnxle : (uint.nat lsnx <= uint.nat (W64 cmd.1))%nat).
+      { rewrite /eq_lsn_last_ilog in Hlsnx.
+        destruct (last iloga) as [[n icmd] |] eqn:Hn; last first.
+        { rewrite Hlsnx. lia. }
+        rewrite last_lookup in Hn.
+        unshelve epose proof (prefix_lookup_Some _ ilog _ _ Hn _) as Hprev.
+        { rewrite Hilogar. by apply prefix_app_r. }
+        assert (Hcur : ilog !! length iloga = Some cmd).
+        { by rewrite Hilogar list_lookup_middle. }
+        rewrite /ilog_lsn_sorted in Hsorted.
+        unshelve epose proof (Hsorted _ _ _ _ _ Hprev Hcur) as Hle.
+        { lia. }
+        simpl in Hle.
+        rewrite -Hlsnx.
+        clear -Hle Hvlsn.
+        word.
+      }
+      wp_apply (wp_Replica__replayBetween with "Hinv Hidx Htxnlog [$Hrp]").
+      { apply Hgid. }
+      { apply Hlelsnx. }
+      { apply Hlsnxle. }
+      iIntros "Hrp".
+
+      (*@         lsnx = lsny                                                     @*)
+      (*@                                                                         @*)
+      wp_store.
+
+      (*@         kind, bs2 := marshal.ReadInt(bs1)                               @*)
+      (*@         ts, bs3 := marshal.ReadInt(bs2)                                 @*)
+      (*@                                                                         @*)
+
+      destruct cmd.2 eqn:Heqcmd.
+      { (* Case: Read. *)
+
+        (*@         if kind == CMD_READ {                                           @*)
+        (*@             key, bs4 := util.DecodeString(bs3)                          @*)
+        (*@             data = bs4                                                  @*)
+        (*@             // Apply read.                                              @*)
+        (*@             rp.bumpKey(ts, key)                                         @*)
+        (*@                                                                         @*)
+        rewrite Henc -2!app_assoc.
+        wp_apply (wp_ReadInt with "Hdata").
+        iIntros (bs2P) "Hdata".
+        wp_apply (wp_ReadInt with "Hdata").
+        iIntros (bs3P) "Hdata".
+        wp_apply (wp_DecodeString with "Hdata").
+        iIntros (bs4P) "Hdata".
+        wp_store.
+        wp_pures.
+        do 2 iNamed "Hrp". rename clog0 into cloga.
+        wp_apply (wp_Replica__bumpKey with "Hptsmsptsm").
+        { rewrite /= /valid_ts in Hvicmd. clear -Hvicmd. word. }
+        { rewrite /= /valid_key in Hvicmd. by destruct Hvicmd as [_ ?]. }
+        iIntros (spts) "[Hptsmsptsm %Hspts]".
+        wp_pures.
+        iApply "HΦ".
+        subst P. simpl.
+        iFrame "HdataPP Hdata HlsnxP".
+        iExists ilogrbs', (iloga ++ [cmd]), ilogr'.
+        iSplitL.
+        { iClear "Hloglb".
+          iFrame "∗ # %".
+          iPureIntro. simpl.
+          exists ptgsm.
+          destruct cmd as [lsn icmd].
+          rewrite merge_clog_ilog_snoc_ilog; last first.
+          { clear -Hlenclog. simpl in Hlenclog. word. }
+          simpl in Heqcmd.
+          rewrite execute_cmds_snoc Heqcmd Hexec /=.
+          rewrite (lookup_alter_Some _ _ _ _ Hspts).
+          do 4 f_equal.
+          (* Prove tid fits in u64 *)
+          rewrite /= /valid_ts in Hvicmd.
+          clear -Hvicmd. word.
+        }
+        iPureIntro.
+        split.
+        { rewrite /eq_lsn_last_ilog last_snoc /=.
+          destruct cmd as [lsn icmd].
+          simpl. simpl in Hvlsn.
+          clear -Hvlsn. word.
+        }
+        split.
+        { apply Forall_app.
+          split.
+          { apply (Forall_impl _ _ _ Hlelsnx). clear -Hlsnxle. lia. }
+          rewrite Forall_singleton. clear -Hvlsn. word.
+        }
+        by rewrite -app_assoc /= Hilogar.
+      }
+      { (* Case: Acquire. *)
+
+        (*@         } else if kind == CMD_ACQUIRE {                                 @*)
+        (*@             pwrs, bs4 := util.DecodeKVMapIntoSlice(bs3)                 @*)
+        (*@             data = bs4                                                  @*)
+        (*@             // Apply validate.                                          @*)
+        (*@             rp.acquire(ts, pwrs)                                        @*)
+        (*@             // TODO: pass @ptgs                                         @*)
+        (*@             rp.memorize(ts, pwrs, nil)                                  @*)
+        (*@                                                                         @*)
+        destruct Henc as [mdata [Hcmddata Hmdata]].
+        rewrite Hcmddata -2!app_assoc.
+        wp_apply (wp_ReadInt with "Hdata").
+        iIntros (bs2P) "Hdata".
+        wp_apply (wp_ReadInt with "Hdata").
+        iIntros (bs3P) "Hdata".
+        wp_apply (wp_DecodeKVMapIntoSlice with "Hdata").
+        { apply Hmdata. }
+        iIntros (pwrsS bs4P) "[Hpwrs Hdata]".
+        wp_store.
+        assert (Hvpwrs : valid_wrs pwrs).
+        { rewrite /= in Hvicmd. by destruct Hvicmd as [_ ?]. }
+        do 2 iNamed "Hrp". rename clog0 into cloga.
+        wp_apply (wp_Replica__acquire with "[$Hpwrs $Hptsmsptsm]").
+        { apply Hvpwrs. }
+        iIntros "[Hpwrs Hptsmsptsm]".
+        wp_apply (wp_Replica__memorize _ _ _ _ Slice.nil with "[$Hpwrs $Hcpm]").
+        iIntros "Hcpm".
+        wp_pures.
+        iApply "HΦ".
+        subst P. simpl.
+        iFrame "HdataPP Hdata HlsnxP".
+        iExists ilogrbs', (iloga ++ [cmd]), ilogr'.
+        iSplitL.
+        { iClear "Hloglb".
+          iFrame "∗ # %".
+          iPureIntro. simpl.
+          exists (<[tid := ptgs]> ptgsm).
+          split.
+          { apply map_Forall_insert_2; [apply Hvpwrs | apply Hvcpm]. }
+          destruct cmd as [lsn icmd].
+          rewrite merge_clog_ilog_snoc_ilog; last first.
+          { clear -Hlenclog. simpl in Hlenclog. word. }
+          simpl in Heqcmd.
+          rewrite execute_cmds_snoc Heqcmd Hexec /=.
+          rewrite uint_nat_W64_of_nat; first done.
+          rewrite /= /valid_ts in Hvicmd.
+          clear -Hvicmd. lia.
+        }
+        iPureIntro.
+        split.
+        { rewrite /eq_lsn_last_ilog last_snoc /=.
+          destruct cmd as [lsn icmd].
+          simpl. simpl in Hvlsn.
+          clear -Hvlsn. word.
+        }
+        split.
+        { apply Forall_app.
+          split.
+          { apply (Forall_impl _ _ _ Hlelsnx). clear -Hlsnxle. lia. }
+          rewrite Forall_singleton. clear -Hvlsn. word.
+        }
+        by rewrite -app_assoc /= Hilogar.
+      }
+      { (* Case: Advance. *)
+
+        (*@         } else if kind == CMD_ADVANCE {                                 @*)
+        (*@             rank, bs4 := marshal.ReadInt(bs3)                           @*)
+        (*@             data = bs4                                                  @*)
+        (*@             rp.advance(ts, rank)                                        @*)
+        (*@                                                                         @*)
+        rewrite Henc -2!app_assoc.
+        wp_apply (wp_ReadInt with "Hdata").
+        iIntros (bs2P) "Hdata".
+        wp_apply (wp_ReadInt with "Hdata").
+        iIntros (bs3P) "Hdata".
+        wp_apply (wp_ReadInt with "Hdata").
+        iIntros (bs4P) "Hdata".
+        wp_store.
+        do 2 iNamed "Hrp". rename clog0 into cloga.
+        wp_apply (wp_Replica__advance with "Hpsmrkm").
+        iIntros "Hpsmrkm".
+        wp_pures.
+        iApply "HΦ".
+        subst P. simpl.
+        iFrame "HdataPP Hdata HlsnxP".
+        iExists ilogrbs', (iloga ++ [cmd]), ilogr'.
+        iSplitL.
+        { iClear "Hloglb".
+          iFrame "∗ # %".
+          iPureIntro. simpl.
+          exists ptgsm.
+          destruct cmd as [lsn icmd].
+          rewrite merge_clog_ilog_snoc_ilog; last first.
+          { clear -Hlenclog. simpl in Hlenclog. word. }
+          simpl in Heqcmd.
+          rewrite execute_cmds_snoc Heqcmd Hexec /=.
+          rewrite /= /valid_ts in Hvicmd.
+          destruct Hvicmd as [Hvtid Hvrank].
+          rewrite uint_nat_W64_of_nat; last word.
+          rewrite uint_nat_W64_of_nat; last word.
+          done.
+        }
+        iPureIntro.
+        split.
+        { rewrite /eq_lsn_last_ilog last_snoc /=.
+          destruct cmd as [lsn icmd].
+          simpl. simpl in Hvlsn.
+          clear -Hvlsn. word.
+        }
+        split.
+        { apply Forall_app.
+          split.
+          { apply (Forall_impl _ _ _ Hlelsnx). clear -Hlsnxle. lia. }
+          rewrite Forall_singleton. clear -Hvlsn. word.
+        }
+        by rewrite -app_assoc /= Hilogar.
+      }
+      { (* Case: Accept. *)
+
+        (*@         } else if kind == CMD_ACCEPT {                                  @*)
+        (*@             rank, bs4 := marshal.ReadInt(bs3)                           @*)
+        (*@             dec, bs5 := marshal.ReadBool(bs4)                           @*)
+        (*@             data = bs5                                                  @*)
+        (*@             // Apply accept.                                            @*)
+        (*@             rp.accept(ts, rank, dec)                                    @*)
+        (*@         }                                                               @*)
+        (*@                                                                         @*)
+        rewrite Henc -2!app_assoc.
+        wp_apply (wp_ReadInt with "Hdata").
+        iIntros (bs2P) "Hdata".
+        wp_apply (wp_ReadInt with "Hdata").
+        iIntros (bs3P) "Hdata".
+        wp_apply (wp_ReadInt with "Hdata").
+        iIntros (bs4P) "Hdata".
+        wp_apply (wp_ReadBool with "Hdata").
+        iIntros (dec bs5P) "[%Hdec Hdata]".
+        wp_store.
+        do 2 iNamed "Hrp". rename clog0 into cloga.
+        wp_apply (wp_Replica__accept with "Hpsmrkm").
+        iIntros "Hpsmrkm".
+        wp_pures.
+        iApply "HΦ".
+        subst P. simpl.
+        iFrame "HdataPP Hdata HlsnxP".
+        iExists ilogrbs', (iloga ++ [cmd]), ilogr'.
+        iSplitL.
+        { iClear "Hloglb".
+          iFrame "∗ # %".
+          iPureIntro. simpl.
+          exists ptgsm.
+          destruct cmd as [lsn icmd].
+          rewrite merge_clog_ilog_snoc_ilog; last first.
+          { clear -Hlenclog. simpl in Hlenclog. word. }
+          simpl in Heqcmd.
+          rewrite execute_cmds_snoc Heqcmd Hexec /=.
+          rewrite /= /valid_ts in Hvicmd.
+          destruct Hvicmd as [Hvtid Hvrank].
+          rewrite uint_nat_W64_of_nat; last word.
+          rewrite uint_nat_W64_of_nat; last word.
+          assert (pdec = dec) as ->.
+          { by destruct dec, pdec. }
+          done.
+        }
+        iPureIntro.
+        split.
+        { rewrite /eq_lsn_last_ilog last_snoc /=.
+          destruct cmd as [lsn icmd].
+          simpl. simpl in Hvlsn.
+          clear -Hvlsn. word.
+        }
+        split.
+        { apply Forall_app.
+          split.
+          { apply (Forall_impl _ _ _ Hlelsnx). clear -Hlsnxle. lia. }
+          rewrite Forall_singleton. clear -Hvlsn. word.
+        }
+        by rewrite -app_assoc /= Hilogar.
+      }
+
+      (*@     }                                                                   @*)
+      (*@                                                                         @*)
+    }
+
+    (*@     rp.lsna = lsnx                                                      @*)
+    (*@ }                                                                       @*)
+    iNamed 1. iNamed "Hrp". rename clog0 into cloga.
+    iNamed "Hlsna".
+    wp_load.
+    wp_storeField.
+    iApply "HΦ".
+    assert (iloga = ilog) as ->.
+    { destruct ilogr as [| c ilogr'].
+      { by rewrite app_nil_r in Hilogar. }
+      exfalso.
+      apply Forall2_cons_inv_l in Hilogr as (bs & ilogrbs' & Henc & _ & Heq).
+      rewrite Heq serialize_cons in Hserial.
+      apply nil_length_inv in Hcont.
+      rewrite Hcont /= in Hserial.
+      destruct bs eqn:Hbs; last done.
+      by apply encode_lsn_icommand_not_nil in Henc.
+    }
+    iDestruct (txn_log_lb_prefix with "Hcloglb Hloglb") as %Horprefix.
+    assert (cloga = clog) as ->.
+    { rewrite /eq_lsn_last_ilog in Hlsnx, Heqlast.
+      destruct (last ilog) as [[n icmd] |].
+      { rewrite -Hlsnx in Hlenclog.
+        destruct Horprefix.
+        { apply prefix_length_eq; [done | lia]. }
+        { symmetry. apply prefix_length_eq; [done | lia]. }
+      }
+      { rewrite Hlsnx in Hlenclog.
+        destruct Horprefix.
+        { apply prefix_length_eq; [done | lia]. }
+        { symmetry. apply prefix_length_eq; [done | lia]. }
+      }
+    }
+    by iFrame.
+  Qed.
+
+End program.
